Pulling more things out

src/SDK/Serialize/SerializableTypes.dfy
@@ -30,4 +30,47 @@ module SerializableTypes {
 
   type ESDKEncryptionContext = ec: EncryptionContext | IsESDKEncryptionContext(ec) witness *
 
+  const VALID_IDS: set<uint16> := {0x0578, 0x0478, 0x0378, 0x0346, 0x0214, 0x0178, 0x0146, 0x0114, 0x0078, 0x0046, 0x0014};
+  
+  type ESDKAlgorithmSuiteId = id: uint16 | id in VALID_IDS witness *
+
+  const SupportedAlgorithmSuites: map<Crypto.AlgorithmSuiteId, ESDKAlgorithmSuiteId> := map[
+    Crypto.AlgorithmSuiteId.ALG_AES_128_GCM_IV12_TAG16_NO_KDF := 0x0014,
+    Crypto.AlgorithmSuiteId.ALG_AES_192_GCM_IV12_TAG16_NO_KDF := 0x0046,
+    Crypto.AlgorithmSuiteId.ALG_AES_256_GCM_IV12_TAG16_NO_KDF := 0x0078,
+    Crypto.AlgorithmSuiteId.ALG_AES_128_GCM_IV12_TAG16_HKDF_SHA256 := 0x0114,
+    Crypto.AlgorithmSuiteId.ALG_AES_192_GCM_IV12_TAG16_HKDF_SHA256 := 0x0146,
+    Crypto.AlgorithmSuiteId.ALG_AES_256_GCM_IV12_TAG16_HKDF_SHA256 := 0x0178,
+    Crypto.AlgorithmSuiteId.ALG_AES_128_GCM_IV12_TAG16_HKDF_SHA256_ECDSA_P256 := 0x0214,
+    Crypto.AlgorithmSuiteId.ALG_AES_192_GCM_IV12_TAG16_HKDF_SHA384_ECDSA_P384 := 0x0346,
+    Crypto.AlgorithmSuiteId.ALG_AES_256_GCM_IV12_TAG16_HKDF_SHA384_ECDSA_P384 := 0x0378,
+    Crypto.AlgorithmSuiteId.ALG_AES_256_GCM_HKDF_SHA512_COMMIT_KEY := 0x0478,
+    Crypto.AlgorithmSuiteId.ALG_AES_256_GCM_HKDF_SHA512_COMMIT_KEY_ECDSA_P384 := 0x0578
+  ]
+
+  function GetESDKAlgorithmSuiteId(
+    suiteId: Crypto.AlgorithmSuiteId
+  ):
+    (res: ESDKAlgorithmSuiteId)
+  {
+    LemmaSupportedAlgorithmSuitesIsComplete(suiteId);
+    SupportedAlgorithmSuites[suiteId]
+  }
+
+  function GetAlgorithmSuiteId(
+    esdkId: ESDKAlgorithmSuiteId
+  ):
+    (res: Crypto.AlgorithmSuiteId)
+  {
+    var suiteId
+    :|
+      && suiteId in SupportedAlgorithmSuites
+      && SupportedAlgorithmSuites[suiteId] == esdkId;
+    suiteId
+  }
+
+  lemma LemmaSupportedAlgorithmSuitesIsComplete(id:Crypto.AlgorithmSuiteId)
+    ensures id in SupportedAlgorithmSuites
+  {}
+
 }
